feat(jose): Ensuring the whole footprint is fresh.

jose_solutions/Ex3.dfy
@@ -6,51 +6,91 @@ module Ex3 {
     var val : nat
     var next : Node?
 
-    ghost var footprint : set<Node>
-    ghost var content : set<nat> 
+    ghost var footprint : set<Node> 
+    ghost var content : set<nat> //set, not list. Which is weird.
 
     ghost function Valid() : bool 
       reads this, this.footprint 
       decreases footprint
     {
-      this in this.footprint 
-      &&
-      if (this.next == null)
-        then 
-          this.footprint == { this }
-          && 
-          this.content == { this.val }
-        else 
-          this.next in this.footprint
-          &&
-          this !in this.next.footprint
-          &&      
-          this.footprint == { this } + this.next.footprint 
-          &&
-          this.content == { this.val } + this.next.content
-          &&
-          this.next.Valid()
+      if (this.next == null) then
+        this.content == { this.val }
+        && this.footprint == { this }
+      else
+        this.next in this.footprint
+        && this.content == { this.val } + this.next.content
+        && this.footprint == { this } + this.next.footprint
+        && this !in next.footprint
+        && this.next.Valid()
     }
 
     constructor (v : nat) 
+      ensures this.Valid()
+      ensures this.content == { v } && this.footprint == { this }
     {
+      this.val := v;
+      this.next := null;
+      this.footprint := { this };
+      this.content := { v };
+
     }
 
     method add(v : nat) returns (r : Node)
+      requires Valid()
+      ensures r.Valid()
+        && r.content== { v } + this.content
+        && r.footprint == { r } + this.footprint
+      ensures fresh(r)
     {
+      r := new Node(v);
+      r.next := this;
+      r.content := { v } + this.content;
+      r.footprint := { r } + this.footprint;
+
     }
 
     method mem(v : nat) returns (b : bool)
+      requires Valid()
+      ensures b == (v in this.content)
     {
+      var curr := this;
+      b := false;
+      ghost var list_aux := {};
+
+      while(curr != null)
+        invariant curr != null ==> curr.Valid()
+        invariant curr != null ==> this.content == list_aux + curr.content
+        invariant curr == null ==> this.content == list_aux
+        decreases if (curr != null) then curr.footprint else {}
+        invariant v !in list_aux
+      {
+        if(curr.val == v){
+          b := true;
+          return;
+        }
+        list_aux := list_aux + { curr.val };
+        curr := curr.next;
+      }
   
     }
-
-    method copy() returns (n : Node)
+    method copy() returns (n : Node) 
+      requires this.Valid()
+      requires this.next != null ==> this.next.Valid()
+      ensures fresh(n.footprint)
+      ensures n.Valid() && n.content == this.content 
+      ensures n.next != null ==> n.footprint - n.next.footprint == { n }
+      ensures n.next == null ==> n.footprint == { n }
+      decreases this.footprint
     {
+      // The constructor already updates the ghost attributes
+      n := new Node(this.val);
+      
+      if (this.next != null) {
+        var aux := this.next.copy();
+        n.next := aux;
+        n.content := { n.val }  + aux.content;
+        n.footprint := { n }  + aux.footprint;
+      }
     }
-
-  
   }
-
-  
 }
